coq/NNRCimpish/Lang/NNRCimpishCrossShadow.v
@@ -1,0 +1,115 @@
+(*
+ * Copyright 2015-2016 IBM Corporation
+ *
+ * Licensed under the Apache License, Version 2.0 (the "License");
+ * you may not use this file except in compliance with the License.
+ * You may obtain a copy of the License at
+ *
+ * http://www.apache.org/licenses/LICENSE-2.0
+ *
+ * Unless required by applicable law or agreed to in writing, software
+ * distributed under the License is distributed on an "AS IS" BASIS,
+ * WITHOUT WARRANTIES OR CONDITIONS OF ANY KIND, either express or implied.
+ * See the License for the specific language governing permissions and
+ * limitations under the License.
+ *)
+
+(* Cross Shadowing is when a variable in one namespace "shadows" 
+   a variable in another namespace.  This is not a problem for nnrc_impish, since 
+   the namespaces are all distinct.  However, it poses a problem when compiling to
+   a language like nnrc_imp that has a single namespace.
+*)
+
+Require Import String.
+Require Import List.
+Require Import Arith.
+Require Import EquivDec.
+Require Import Morphisms.
+Require Import Arith.
+Require Import Max.
+Require Import Bool.
+Require Import Peano_dec.
+Require Import EquivDec.
+Require Import Decidable.
+Require Import Utils.
+Require Import CommonRuntime.
+Require Import NNRCimpish.
+Require Import NNRCimpishVars.
+
+Section NNRCimpishCrossShadow.
+
+  Context {fruntime:foreign_runtime}.
+
+  Context (h:brand_relation_t).
+
+  Local Open Scope nnrc_impish.
+  Local Open Scope string.
+
+  Fixpoint nnrc_impish_stmt_cross_shadow_free_under
+           (s:nnrc_impish_stmt)
+           (σ ψc ψd:list var)
+    : Prop
+    := match s with
+       | NNRCimpishSeq s₁ s₂ =>
+         nnrc_impish_stmt_cross_shadow_free_under s₁ σ ψc ψd
+         /\ nnrc_impish_stmt_cross_shadow_free_under s₂ σ ψc ψd
+       | NNRCimpishLet v e s₀ =>
+         disjoint (nnrc_impish_expr_free_vars e) ψc
+         /\ disjoint (nnrc_impish_expr_free_vars e) ψd
+        (* not the same: incl (nnrc_impish_expr_free_vars e) σ *)
+         /\ ~ In v ψc
+         /\ ~ In v ψd
+         /\ nnrc_impish_stmt_cross_shadow_free_under s₀ (v::σ) ψc ψd
+       | NNRCimpishLetMut v s₁ s₂ =>
+            ~ In v σ
+         /\ ~ In v ψc
+         /\ ~ In v ψd      
+         /\ nnrc_impish_stmt_cross_shadow_free_under s₁ σ ψc (v::ψd)
+         /\ nnrc_impish_stmt_cross_shadow_free_under s₂ (v::σ) ψc ψd
+       | NNRCimpishLetMutColl v s₁ s₂ =>
+            ~ In v σ
+         /\ ~ In v ψc
+         /\ ~ In v ψd      
+         /\ nnrc_impish_stmt_cross_shadow_free_under s₁ σ (v::ψc) ψd
+         /\ nnrc_impish_stmt_cross_shadow_free_under s₂ (v::σ) ψc ψd
+       | NNRCimpishAssign v e =>
+            disjoint (nnrc_impish_expr_free_vars e) ψc
+         /\ disjoint (nnrc_impish_expr_free_vars e) ψd
+         /\ ~ In v σ
+         /\ ~ In v ψc
+       (* not the same: In v ψd *)
+       | NNRCimpishPush v e =>
+         disjoint (nnrc_impish_expr_free_vars e) ψc
+         /\ disjoint (nnrc_impish_expr_free_vars e) ψd
+         /\ ~ In v σ
+         /\ ~ In v ψd
+       (* not the same: In v ψc *)
+       | NNRCimpishFor v e s₀ =>
+         disjoint (nnrc_impish_expr_free_vars e) ψc
+         /\ disjoint (nnrc_impish_expr_free_vars e) ψd
+        (* not the same: incl (nnrc_impish_expr_free_vars e) σ *)          
+         /\ ~ In v ψc
+         /\ ~ In v ψd
+         /\ nnrc_impish_stmt_cross_shadow_free_under s₀ (v::σ) ψc ψd
+       | NNRCimpishIf e s₁ s₂ =>
+         disjoint (nnrc_impish_expr_free_vars e) ψc
+         /\ disjoint (nnrc_impish_expr_free_vars e) ψd
+        (* not the same: incl (nnrc_impish_expr_free_vars e) σ *)
+         /\ nnrc_impish_stmt_cross_shadow_free_under s₁ σ ψc ψd
+         /\ nnrc_impish_stmt_cross_shadow_free_under s₂ σ ψc ψd
+       | NNRCimpishEither e x₁ s₁ x₂ s₂ =>
+         disjoint (nnrc_impish_expr_free_vars e) ψc
+         /\ disjoint (nnrc_impish_expr_free_vars e) ψd
+        (* not the same: incl (nnrc_impish_expr_free_vars e) σ *)
+         /\ ~ In x₁ ψc
+         /\ ~ In x₁ ψd
+         /\ ~ In x₂ ψc
+         /\ ~ In x₂ ψd
+         /\ nnrc_impish_stmt_cross_shadow_free_under s₁ (x₁::σ) ψc ψd
+         /\ nnrc_impish_stmt_cross_shadow_free_under s₂ (x₂::σ) ψc ψd
+       end.
+
+  Definition nnrc_impish_cross_shadow_free (s:nnrc_impish)
+    := nnrc_impish_stmt_cross_shadow_free_under (fst s) nil nil (snd s::nil).
+  
+End NNRCimpishCrossShadow.
