coq/NNRCimpish/Lang/NNRCimpishVars.v
@@ -43,4 +43,70 @@ Section NNRCimpishVars.
        | NNRCimpishGroupBy _ _ e₁ => nnrc_impish_expr_free_vars e₁
        end.
 
+  Fixpoint nnrc_impish_stmt_bound_env_vars (s:nnrc_impish_stmt) : list var
+    := match s with
+       | NNRCimpishSeq s₁ s₂ =>
+         nnrc_impish_stmt_bound_env_vars s₁ ++ nnrc_impish_stmt_bound_env_vars s₂
+       | NNRCimpishLet v e s₀ =>
+         v :: nnrc_impish_stmt_bound_env_vars s₀
+       | NNRCimpishLetMut v s₁ s₂ =>
+         v :: nnrc_impish_stmt_bound_env_vars s₁ ++ nnrc_impish_stmt_bound_env_vars s₂
+       | NNRCimpishLetMutColl v s₁ s₂ =>
+         v :: nnrc_impish_stmt_bound_env_vars s₁ ++ nnrc_impish_stmt_bound_env_vars s₂
+       | NNRCimpishAssign v e =>
+         nil
+       | NNRCimpishPush v e =>
+         nil
+       | NNRCimpishFor v e s₀ =>
+         v :: nnrc_impish_stmt_bound_env_vars s₀
+       | NNRCimpishIf e s₁ s₂ =>
+         nnrc_impish_stmt_bound_env_vars s₁ ++ nnrc_impish_stmt_bound_env_vars s₂
+       | NNRCimpishEither e x₁ s₁ x₂ s₂ =>
+         x₁ :: x₂ :: nnrc_impish_stmt_bound_env_vars s₁ ++ nnrc_impish_stmt_bound_env_vars s₂
+       end.
+
+  Fixpoint nnrc_impish_stmt_bound_mcenv_vars (s:nnrc_impish_stmt) : list var
+    := match s with
+       | NNRCimpishSeq s₁ s₂ =>
+         nnrc_impish_stmt_bound_mcenv_vars s₁ ++ nnrc_impish_stmt_bound_mcenv_vars s₂
+       | NNRCimpishLet v e s₀ =>
+         nnrc_impish_stmt_bound_mcenv_vars s₀
+       | NNRCimpishLetMut v s₁ s₂ =>
+         nnrc_impish_stmt_bound_mcenv_vars s₁ ++ nnrc_impish_stmt_bound_mcenv_vars s₂
+       | NNRCimpishLetMutColl v s₁ s₂ =>
+         v :: nnrc_impish_stmt_bound_mcenv_vars s₁ ++ nnrc_impish_stmt_bound_mcenv_vars s₂
+       | NNRCimpishAssign v e =>
+         nil
+       | NNRCimpishPush v e =>
+         nil
+       | NNRCimpishFor v e s₀ =>
+         nnrc_impish_stmt_bound_mcenv_vars s₀
+       | NNRCimpishIf e s₁ s₂ =>
+         nnrc_impish_stmt_bound_mcenv_vars s₁ ++ nnrc_impish_stmt_bound_mcenv_vars s₂
+       | NNRCimpishEither e x₁ s₁ x₂ s₂ =>
+         nnrc_impish_stmt_bound_mcenv_vars s₁ ++ nnrc_impish_stmt_bound_mcenv_vars s₂
+       end.
+
+    Fixpoint nnrc_impish_stmt_bound_mdenv_vars (s:nnrc_impish_stmt) : list var
+    := match s with
+       | NNRCimpishSeq s₁ s₂ =>
+         nnrc_impish_stmt_bound_mdenv_vars s₁ ++ nnrc_impish_stmt_bound_mdenv_vars s₂
+       | NNRCimpishLet v e s₀ =>
+         nnrc_impish_stmt_bound_mdenv_vars s₀
+       | NNRCimpishLetMut v s₁ s₂ =>
+         v :: nnrc_impish_stmt_bound_mdenv_vars s₁ ++ nnrc_impish_stmt_bound_mdenv_vars s₂
+       | NNRCimpishLetMutColl v s₁ s₂ =>
+         nnrc_impish_stmt_bound_mdenv_vars s₁ ++ nnrc_impish_stmt_bound_mdenv_vars s₂
+       | NNRCimpishAssign v e =>
+         nil
+       | NNRCimpishPush v e =>
+         nil
+       | NNRCimpishFor v e s₀ =>
+         nnrc_impish_stmt_bound_mdenv_vars s₀
+       | NNRCimpishIf e s₁ s₂ =>
+         nnrc_impish_stmt_bound_mdenv_vars s₁ ++ nnrc_impish_stmt_bound_mdenv_vars s₂
+       | NNRCimpishEither e x₁ s₁ x₂ s₂ =>
+         nnrc_impish_stmt_bound_mdenv_vars s₁ ++ nnrc_impish_stmt_bound_mdenv_vars s₂
+         end.
+  
 End NNRCimpishVars.
