coq/Translation/NNRCimpishtoNNRCimp.v
@@ -1,0 +1,841 @@
+(*
+ * Copyright 2015-2016 IBM Corporation
+ *
+ * Licensed under the Apache License, Version 2.0 (the "License");
+ * you may not use this file except in compliance with the License.
+ * You may obtain a copy of the License at
+ *
+ * http://www.apache.org/licenses/LICENSE-2.0
+ *
+ * Unless required by applicable law or agreed to in writing, software
+ * distributed under the License is distributed on an "AS IS" BASIS,
+ * WITHOUT WARRANTIES OR CONDITIONS OF ANY KIND, either express or implied.
+ * See the License for the specific language governing permissions and
+ * limitations under the License.
+ *)
+
+Require Import String.
+Require Import List.
+Require Import Bool.
+Require Import Arith.
+Require Import EquivDec.
+Require Import Morphisms.
+Require Import Permutation.
+Require Import Eqdep_dec.
+Require Import Program.    
+
+Require Import Utils.
+Require Import CommonRuntime.
+Require Import NNRCimpishRuntime.
+Require Import NNRCimpRuntime.
+Require Import NNRCimpishCrossShadow.
+Require Import Fresh.
+
+Section NNRCimpishtoNNRCimp.
+
+  Context {fruntime:foreign_runtime}.
+
+  Fixpoint nnrc_impish_expr_to_nnrc_imp_expr (e: nnrc_impish_expr) : nnrc_imp_expr
+    := match e with
+       | NNRCimpishGetConstant v =>
+         NNRCimpGetConstant v
+       | NNRCimpishVar v =>
+         NNRCimpVar v
+       | NNRCimpishConst d =>
+         NNRCimpConst d
+       | NNRCimpishBinop bop e₁ e₂ =>
+         NNRCimpBinop bop
+                      (nnrc_impish_expr_to_nnrc_imp_expr e₁)
+                      (nnrc_impish_expr_to_nnrc_imp_expr e₂)
+       | NNRCimpishUnop uop e =>
+         NNRCimpUnop uop
+                     (nnrc_impish_expr_to_nnrc_imp_expr e)
+       | NNRCimpishGroupBy g sl e =>
+         NNRCimpGroupBy g sl
+                        (nnrc_impish_expr_to_nnrc_imp_expr e)
+       end.
+
+  Lemma nnrc_impish_expr_to_nnrc_imp_expr_correct (e:nnrc_impish_expr) :
+    forall h σc σ,
+      nnrc_impish_expr_eval h σc σ e =
+      nnrc_imp_expr_eval h σc
+                         σ
+                         (nnrc_impish_expr_to_nnrc_imp_expr e) .
+  Proof.
+    induction e; intros h σc σ; simpl; trivial
+    ; try rewrite IHe
+    ; try rewrite IHe1
+    ; try rewrite IHe2
+    ; trivial.
+  Qed.
+
+  Fixpoint nnrc_impish_stmt_to_nnrc_imp_stmt (s: nnrc_impish_stmt)
+    : nnrc_imp_stmt
+    := match s with
+       | NNRCimpishSeq s₁ s₂ =>
+         NNRCimpSeq
+           (nnrc_impish_stmt_to_nnrc_imp_stmt s₁)
+           (nnrc_impish_stmt_to_nnrc_imp_stmt s₂)
+       | NNRCimpishLet v e s₀ =>
+         NNRCimpLet v
+                    (Some (nnrc_impish_expr_to_nnrc_imp_expr e))
+                    (nnrc_impish_stmt_to_nnrc_imp_stmt s₀)
+       | NNRCimpishLetMut v s₁ s₂ =>
+         NNRCimpLet v
+                    None
+                    (NNRCimpSeq
+                       (nnrc_impish_stmt_to_nnrc_imp_stmt s₁)
+                       (nnrc_impish_stmt_to_nnrc_imp_stmt s₂))
+       | NNRCimpishLetMutColl v s₁ s₂ =>
+         NNRCimpLet v
+                    (Some (NNRCimpConst (dcoll nil)))
+                    (NNRCimpSeq
+                       (nnrc_impish_stmt_to_nnrc_imp_stmt s₁)
+                       (nnrc_impish_stmt_to_nnrc_imp_stmt s₂))
+       | NNRCimpishAssign v e =>
+         NNRCimpAssign v
+                       (nnrc_impish_expr_to_nnrc_imp_expr e)
+       | NNRCimpishPush v e =>
+         NNRCimpAssign v
+                       (NNRCimpBinop OpBagUnion
+                                     (NNRCimpVar v)
+                                     (NNRCimpUnop OpBag (nnrc_impish_expr_to_nnrc_imp_expr e)))
+       | NNRCimpishFor v e s₀ =>
+         NNRCimpFor v
+                    (nnrc_impish_expr_to_nnrc_imp_expr e)
+                    (nnrc_impish_stmt_to_nnrc_imp_stmt s₀)
+       | NNRCimpishIf e s₁ s₂ =>
+         NNRCimpIf
+           (nnrc_impish_expr_to_nnrc_imp_expr e)
+           (nnrc_impish_stmt_to_nnrc_imp_stmt s₁)
+           (nnrc_impish_stmt_to_nnrc_imp_stmt s₂)           
+       | NNRCimpishEither e x₁ s₁ x₂ s₂ =>
+         NNRCimpEither
+           (nnrc_impish_expr_to_nnrc_imp_expr e)
+           x₁ (nnrc_impish_stmt_to_nnrc_imp_stmt s₁)
+           x₂ (nnrc_impish_stmt_to_nnrc_imp_stmt s₂)
+       end.
+
+  Definition nnrc_impish_to_nnrc_imp (s: nnrc_impish)
+    : nnrc_imp
+    := (nnrc_impish_stmt_to_nnrc_imp_stmt (fst s), snd s).
+
+  Definition pd_bindings := list (string*option data).
+  Definition mc_bindings := list (string*list data).
+  Definition md_bindings := list (string*option data).
+
+  
+  (*
+    Require Import Interleaved.
+  Lemma nnrc_imp_stmt_eval_close_enough h σc σ₁ σ₂ s :
+    close_enough_envs σ₁ σ₂ ->
+    lift2P close_enough_envs
+           (nnrc_imp_stmt_eval h σc s σ₁) (nnrc_imp_stmt_eval h σc s σ₂).
+  Proof.
+    revert σ₁ σ₂.
+    nnrc_imp_stmt_cases (induction s) Case
+    ; simpl; intros σ₁ σ₂ ceq.
+    - Case "NNRCimpSeq"%string.
+      generalize (IHs1 _ _ ceq)
+      ; intros ceq1.
+      unfold lift2P in ceq1; repeat match_option_in ceq1; simpl; try contradiction.
+      eauto.
+    - Case "NNRCimpAssign"%string.
+      repeat rewrite (close_enough_envs_lookup_equiv _ _ ceq).
+      repeat match_destr; simpl; trivial.
+      apply close_enough_update_first; trivial.
+    - Case "NNRCimpLet"%string.
+      destruct o.
+      + rewrite (close_enough_envs_lookup_equiv _ _ ceq).
+        destruct (nnrc_imp_expr_eval h σc σ₂ n); simpl; trivial.
+        assert (ceq1cons: close_enough_envs ((v,Some d)::σ₁) ((v,Some d)::σ₂)).
+        { apply close_enough_envs_cons; trivial. }
+        specialize (IHs _ _ ceq1cons).
+        unfold lift2P in IHs; repeat match_option_in IHs; simpl; try contradiction.
+        generalize (nnrc_imp_stmt_eval_env_domain_stack eqq); simpl; intros domeqq.
+        destruct p; simpl in domeqq; invcs domeqq.
+        generalize (nnrc_imp_stmt_eval_env_domain_stack eqq0); simpl; intros domeqq'.
+        destruct p0; simpl in domeqq'; invcs domeqq'.
+        destruct p; destruct p0; simpl in *; subst.
+        apply close_enough_envs_cons_invs in IHs; tauto.
+      + assert (ceq1cons: close_enough_envs ((v,None)::σ₁) ((v,None)::σ₂)).
+        { apply close_enough_envs_cons; trivial. }
+        specialize (IHs _ _ ceq1cons).
+        unfold lift2P in IHs; repeat match_option_in IHs; simpl; try contradiction.
+        generalize (nnrc_imp_stmt_eval_env_domain_stack eqq); simpl; intros domeqq.
+        destruct p; simpl in domeqq; invcs domeqq.
+        generalize (nnrc_imp_stmt_eval_env_domain_stack eqq0); simpl; intros domeqq'.
+        destruct p0; simpl in domeqq'; invcs domeqq'.
+        destruct p; destruct p0; simpl in *; subst.
+        apply close_enough_envs_cons_invs in IHs; tauto.
+    - Case "NNRCimpFor"%string.
+      rewrite (close_enough_envs_lookup_equiv _ _ ceq).
+      match_option; simpl; trivial.
+      destruct d; simpl; trivial.
+      clear n eqq.
+      revert σ₁ σ₂ ceq.
+      induction l; intros σ₁ σ₂ ceq.
+      + simpl; trivial.
+      + assert (ceq1cons: close_enough_envs ((v,Some a)::σ₁) ((v,Some a)::σ₂)).
+        { apply close_enough_envs_cons; trivial. }
+        specialize (IHs _ _ ceq1cons).
+        unfold lift2P in IHs; repeat match_option_in IHs; simpl; try contradiction.
+        generalize (nnrc_imp_stmt_eval_env_domain_stack eqq); simpl; intros domeqq.
+        destruct p; simpl in domeqq; invcs domeqq.
+        generalize (nnrc_imp_stmt_eval_env_domain_stack eqq0); simpl; intros domeqq'.
+        destruct p0; simpl in domeqq'; invcs domeqq'.
+        destruct p; destruct p0; simpl in *; subst.
+        apply close_enough_envs_cons_invs in IHs.
+        destruct IHs as [? IHs]; subst.
+        eauto.
+    - Case "NNRCimpIf"%string.
+      rewrite (close_enough_envs_lookup_equiv _ _ ceq).
+      match_destr; simpl; trivial.
+      destruct d; simpl; trivial.
+      destruct b; simpl; eauto.
+    - rewrite (close_enough_envs_lookup_equiv _ _ ceq).
+      match_destr; simpl; trivial.
+      destruct d; simpl; trivial.
+      + assert (ceq1cons: close_enough_envs ((v,Some d)::σ₁) ((v,Some d)::σ₂)).
+        { apply close_enough_envs_cons; trivial. }
+        specialize (IHs1 _ _ ceq1cons).
+        unfold lift2P in IHs1; repeat match_option_in IHs1; simpl; try contradiction.
+        generalize (nnrc_imp_stmt_eval_env_domain_stack eqq); simpl; intros domeqq.
+        destruct p; simpl in domeqq; invcs domeqq.
+        generalize (nnrc_imp_stmt_eval_env_domain_stack eqq0); simpl; intros domeqq'.
+        destruct p0; simpl in domeqq'; invcs domeqq'.
+        destruct p; destruct p0; simpl in *; subst.
+        apply close_enough_envs_cons_invs in IHs1.
+        tauto.
+      + assert (ceq1cons: close_enough_envs ((v0,Some d)::σ₁) ((v0,Some d)::σ₂)).
+        { apply close_enough_envs_cons; trivial. }
+        specialize (IHs2 _ _ ceq1cons).
+        unfold lift2P in IHs2; repeat match_option_in IHs2; simpl; try contradiction.
+        generalize (nnrc_imp_stmt_eval_env_domain_stack eqq); simpl; intros domeqq.
+        destruct p; simpl in domeqq; invcs domeqq.
+        generalize (nnrc_imp_stmt_eval_env_domain_stack eqq0); simpl; intros domeqq'.
+        destruct p0; simpl in domeqq'; invcs domeqq'.
+        destruct p; destruct p0; simpl in *; subst.
+        apply close_enough_envs_cons_invs in IHs2.
+        tauto.
+  Qed.
+   *)
+  
+  Lemma nnrc_imp_stmt_eval_grouped_equiv {σ₁ σ₂} :
+    grouped_equiv σ₁ σ₂ ->
+    forall h σc s,
+      lift2P grouped_equiv
+             (nnrc_imp_stmt_eval h σc s σ₁) (nnrc_imp_stmt_eval h σc s σ₂).
+  Proof.
+    intros ceq h σc s.
+    revert σ₁ σ₂ ceq.
+    nnrc_imp_stmt_cases (induction s) Case
+    ; simpl; intros σ₁ σ₂ ceq.
+    - Case "NNRCimpSeq"%string.
+      generalize (IHs1 _ _ ceq)
+      ; intros ceq1.
+      unfold lift2P in ceq1; repeat match_option_in ceq1; simpl; try contradiction.
+      eauto.
+    - Case "NNRCimpAssign"%string.
+      repeat rewrite (grouped_equiv_lookup_equiv _ _ ceq).
+      unfold var, string_eqdec.
+      repeat match_destr; simpl; trivial.
+      apply grouped_equiv_update_first; trivial.
+    - Case "NNRCimpLet"%string.
+      destruct o.
+      + rewrite (grouped_equiv_lookup_equiv _ _ ceq).
+        destruct (nnrc_imp_expr_eval h σc σ₂ n); simpl; trivial.
+        assert (ceq1cons: grouped_equiv ((v,Some d)::σ₁) ((v,Some d)::σ₂)).
+        { apply grouped_equiv_cons; trivial. }
+        specialize (IHs _ _ ceq1cons).
+        unfold lift2P in IHs; repeat match_option_in IHs; simpl; try contradiction.
+        generalize (nnrc_imp_stmt_eval_env_domain_stack eqq); simpl; intros domeqq.
+        destruct p; simpl in domeqq; invcs domeqq.
+        generalize (nnrc_imp_stmt_eval_env_domain_stack eqq0); simpl; intros domeqq'.
+        destruct p0; simpl in domeqq'; invcs domeqq'.
+        destruct p; destruct p0; simpl in *; subst.
+        apply grouped_equiv_cons_invs in IHs; tauto.
+      + assert (ceq1cons: grouped_equiv ((v,None)::σ₁) ((v,None)::σ₂)).
+        { apply grouped_equiv_cons; trivial. }
+        specialize (IHs _ _ ceq1cons).
+        unfold lift2P in IHs; repeat match_option_in IHs; simpl; try contradiction.
+        generalize (nnrc_imp_stmt_eval_env_domain_stack eqq); simpl; intros domeqq.
+        destruct p; simpl in domeqq; invcs domeqq.
+        generalize (nnrc_imp_stmt_eval_env_domain_stack eqq0); simpl; intros domeqq'.
+        destruct p0; simpl in domeqq'; invcs domeqq'.
+        destruct p; destruct p0; simpl in *; subst.
+        apply grouped_equiv_cons_invs in IHs; tauto.
+    - Case "NNRCimpFor"%string.
+      rewrite (grouped_equiv_lookup_equiv _ _ ceq).
+      match_option; simpl; trivial.
+      destruct d; simpl; trivial.
+      clear n eqq.
+      revert σ₁ σ₂ ceq.
+      induction l; intros σ₁ σ₂ ceq.
+      + simpl; trivial.
+      + assert (ceq1cons: grouped_equiv ((v,Some a)::σ₁) ((v,Some a)::σ₂)).
+        { apply grouped_equiv_cons; trivial. }
+        specialize (IHs _ _ ceq1cons).
+        unfold lift2P in IHs; repeat match_option_in IHs; simpl; try contradiction.
+        generalize (nnrc_imp_stmt_eval_env_domain_stack eqq); simpl; intros domeqq.
+        destruct p; simpl in domeqq; invcs domeqq.
+        generalize (nnrc_imp_stmt_eval_env_domain_stack eqq0); simpl; intros domeqq'.
+        destruct p0; simpl in domeqq'; invcs domeqq'.
+        destruct p; destruct p0; simpl in *; subst.
+        apply grouped_equiv_cons_invs in IHs.
+        destruct IHs as [? IHs]; subst.
+        eauto.
+    - Case "NNRCimpIf"%string.
+      rewrite (grouped_equiv_lookup_equiv _ _ ceq).
+      match_destr; simpl; trivial.
+      destruct d; simpl; trivial.
+      destruct b; simpl; eauto.
+    - rewrite (grouped_equiv_lookup_equiv _ _ ceq).
+      match_destr; simpl; trivial.
+      destruct d; simpl; trivial.
+      + assert (ceq1cons: grouped_equiv ((v,Some d)::σ₁) ((v,Some d)::σ₂)).
+        { apply grouped_equiv_cons; trivial. }
+        specialize (IHs1 _ _ ceq1cons).
+        unfold lift2P in IHs1; repeat match_option_in IHs1; simpl; try contradiction.
+        generalize (nnrc_imp_stmt_eval_env_domain_stack eqq); simpl; intros domeqq.
+        destruct p; simpl in domeqq; invcs domeqq.
+        generalize (nnrc_imp_stmt_eval_env_domain_stack eqq0); simpl; intros domeqq'.
+        destruct p0; simpl in domeqq'; invcs domeqq'.
+        destruct p; destruct p0; simpl in *; subst.
+        apply grouped_equiv_cons_invs in IHs1.
+        tauto.
+      + assert (ceq1cons: grouped_equiv ((v0,Some d)::σ₁) ((v0,Some d)::σ₂)).
+        { apply grouped_equiv_cons; trivial. }
+        specialize (IHs2 _ _ ceq1cons).
+        unfold lift2P in IHs2; repeat match_option_in IHs2; simpl; try contradiction.
+        generalize (nnrc_imp_stmt_eval_env_domain_stack eqq); simpl; intros domeqq.
+        destruct p; simpl in domeqq; invcs domeqq.
+        generalize (nnrc_imp_stmt_eval_env_domain_stack eqq0); simpl; intros domeqq'.
+        destruct p0; simpl in domeqq'; invcs domeqq'.
+        destruct p; destruct p0; simpl in *; subst.
+        apply grouped_equiv_cons_invs in IHs2.
+        tauto.
+  Qed.
+  
+
+  Ltac preserve_doms :=
+    unfold var in *
+    ; repeat progress
+             match goal with
+             | [H : nnrc_impish_stmt_eval ?h ?σc ?σ₁ ?ψc₁ ?ψd₁ ?s = Some (?σ₂, _, _) |- _ ] =>
+               generalize (nnrc_impish_stmt_eval_env_stack H); intros ?; subst σ₂
+               ; repeat rewrite (nnrc_impish_stmt_eval_mcenv_domain_stack H) in *
+               ; repeat rewrite (nnrc_impish_stmt_eval_mdenv_domain_stack H) in *
+             | [H : nnrc_impish_stmt_eval ?h ?σc ?σ₁ ?ψc₁ ?ψd₁ ?s = Some _ |- _ ] =>
+               repeat rewrite (nnrc_impish_stmt_eval_env_domain_stack H) in *
+               ; repeat rewrite (nnrc_impish_stmt_eval_mcenv_domain_stack H) in *
+               ; repeat rewrite (nnrc_impish_stmt_eval_mdenv_domain_stack H) in *
+             end.
+
+  (* The hard part is that the environments produced are not actually equal,
+       rather, o     ne is an interleaved version of the other.
+       This is capt  ured via the is_interleaved predicate.
+   *)
+  
+  Definition concat_envs (envs:pd_bindings*mc_bindings*md_bindings)
+    : pd_bindings
+    := let '(σ, ψc, ψd) := envs in
+       σ++(map_codomain (fun x => Some (dcoll x)) ψc)++ψd.
+
+  (* hm. Maybe we should use lookup_equiv instead of Permutation in the definition 
+     of grouped_equiv, since they are equivalent in this case *)
+  Lemma grouped_equiv_move_to_front {A B} {dec:EqDec A eq} (l1 : list (list (A*B))) a l2 l3:
+    ~ In (fst a) (domain (concat l1)) ->
+    (grouped_equiv
+       (concat (l1++(a::l2)::l3))
+       (a::concat (l1++l2::l3))).
+  Proof.
+    destruct a; simpl.
+    intros nin.
+    unfold grouped_equiv.
+    apply NoDup_lookup_equiv_Permutation
+    ; try apply groupby_domain_NoDup.
+    simpl.
+    repeat rewrite concat_app; simpl.
+    unfold lookup_equiv; intros x.
+    destruct (a == x); unfold equiv, complement in *.
+    - subst.
+      generalize (groupby_domain_lookup_app_nin nil (concat l1)); simpl; intros re.
+      repeat rewrite re by trivial; simpl.
+      match_destr.
+      + replace dec with (@equiv_dec _ _ _ dec) in * by trivial.
+        destruct (in_dec dec x (domain ((groupby_domain (l2 ++ concat l3))))).
+        * repeat rewrite lookup_update_eq_in; trivial.
+          rewrite groupby_domain_equivlist in *.
+          repeat rewrite domain_app, in_app_iff in *; tauto.
+        * repeat rewrite lookup_nin_none; trivial
+          ; rewrite domain_update_first; trivial.
+          rewrite groupby_domain_equivlist in *.
+          repeat rewrite domain_app, in_app_iff in *; tauto.
+      + simpl; match_destr; congruence.
+    - generalize (groupby_domain_lookup_app_nin (concat l1) ((a,b)::nil)); simpl; intros re.
+      rewrite re by tauto.
+      match_option.
+      + replace dec with (@equiv_dec _ _ _ dec) in * by trivial.
+        rewrite lookup_update_neq by congruence.
+        trivial.
+      + simpl.
+        match_destr; congruence.
+  Qed.
+
+
+  Lemma grouped_equiv_mcenv_env a l1 l2 l3:
+    ~ In (fst a) (domain l1) ->
+    (grouped_equiv
+       (concat_envs (l1,a::l2,l3))
+       (concat_envs ((fst a, Some (dcoll (snd a)))::l1,l2,l3))).
+  Proof.
+    unfold concat_envs; simpl.
+    intros nin.
+    generalize (grouped_equiv_move_to_front (l1::nil) (fst a, Some (dcoll (snd a)))
+                                            (map_codomain (fun x : list data => Some (dcoll x)) l2) (l3::nil)); simpl.
+    repeat rewrite app_nil_r.
+    auto.
+  Qed.
+  
+  Lemma grouped_equiv_mdenv_env a l1 l2 l3:
+    ~ In (fst a) (domain l1) ->
+    ~ In (fst a) (domain l2) ->
+    (grouped_equiv
+       (concat_envs (l1,l2,a::l3))
+       (concat_envs (a::l1,l2,l3))).
+  Proof.
+    unfold concat_envs; simpl.
+    intros nin1 nin2.
+    generalize (grouped_equiv_move_to_front (l1::(map_codomain (fun x : list data => Some (dcoll x)) l2)::nil) a l3 nil); simpl.
+    repeat rewrite app_nil_r.
+    intros re; apply re.
+    rewrite domain_app, domain_map_codomain, in_app_iff.
+    tauto.
+  Qed.
+
+  Lemma nnrc_impish_stmt_to_nnrc_imp_stmt_correct (s:nnrc_impish_stmt) :
+    forall h σc σ ψc ψd,
+      nnrc_impish_stmt_cross_shadow_free_under s (domain σ) (domain ψc) (domain ψd)->
+      all_disjoint ((domain σ)::(domain ψc)::(domain ψd)::nil) ->
+      lift2P grouped_equiv
+             (lift concat_envs
+                   (nnrc_impish_stmt_eval h σc σ ψc ψd s))
+             (nnrc_imp_stmt_eval h σc
+                                 (nnrc_impish_stmt_to_nnrc_imp_stmt s) 
+                                 (concat_envs (σ, ψc, ψd))).
+  Proof.
+    unfold concat_envs.
+    intros h σc.
+    nnrc_impish_stmt_cases (induction s) Case
+    ; simpl; intros σ ψc ψd sf disj.
+    - Case "NNRCimpishSeq"%string.
+      destruct sf as [sf1 sf2].
+      specialize (IHs1 _ _ _ sf1 disj).
+      unfold lift2P in IHs1; repeat match_option_in IHs1; try contradiction; simpl in *.
+      + apply some_lift in eqq.
+        destruct eqq as [[[??]?] eqq ?]; subst.
+        rewrite eqq.
+        preserve_doms.
+        rewrite (IHs2 _ _ _ sf2 disj).
+        rewrite (nnrc_imp_stmt_eval_grouped_equiv IHs1).
+        reflexivity.
+      + apply none_lift in eqq.
+        rewrite eqq; simpl; trivial.
+    - Case "NNRCimpishLet"%string.
+      destruct sf as [disj1 [disj2 [nin1 [nin2 sf]]]].
+      rewrite <- (nnrc_impish_expr_to_nnrc_imp_expr_correct n).
+      rewrite nnrc_impish_expr_eval_free_env, nnrc_impish_expr_eval_free_env_tail
+        by (try rewrite domain_map_codomain; tauto).
+      match_option; simpl; trivial.
+      specialize (IHs ((v, Some d)::σ) ψc ψd); simpl in IHs.
+      cut_to IHs; trivial.
+      + match_option
+        ; rewrite eqq0 in IHs; simpl in *.
+        * destruct p as [[??]?].
+          match_option
+          ; unfold var in *; rewrite eqq1 in IHs
+          ; try contradiction.
+          preserve_doms; simpl.
+          generalize (nnrc_imp_stmt_eval_env_domain_stack eqq1).
+          destruct p0; simpl; intros deq; invcs deq.
+          destruct p; simpl in IHs.
+          apply grouped_equiv_cons_invs in IHs.
+          tauto.
+        * match_option_in IHs; try contradiction.
+          unfold var in *; rewrite eqq1; trivial.
+      + rewrite all_disjoint3_iff in *.
+        repeat split; try tauto
+        ; apply disjoint_cons1; tauto.
+    - Case "NNRCimpishLetMut"%string.
+      destruct sf as [nin1 [nin2 [nin3 [sf1 sf2]]]].
+      specialize (IHs1 _ _ ((v, None)::ψd) sf1).
+      cut_to IHs1; [ | 
+                     rewrite all_disjoint3_iff in *
+                     ; repeat split; try tauto
+                     ; apply disjoint_cons2; tauto].
+      unfold lift2P in IHs1.
+      repeat match_option_in IHs1; try contradiction.
+      + apply some_lift in eqq.
+        destruct eqq as [[[??]?] eqq ?]; subst.
+        rewrite eqq.
+        preserve_doms.
+        generalize (nnrc_impish_stmt_eval_mdenv_domain_stack eqq)
+        ; destruct m0; intros deq; invcs deq.
+        destruct p; simpl in *.
+        generalize (grouped_equiv_mdenv_env (s,None) σ ψc ψd); simpl
+        ; intros geq1.
+        generalize (grouped_equiv_mdenv_env (s,o) σ m m0); simpl
+        ; intros geq2.
+        rewrite geq2 in IHs1 by trivial.
+        preserve_doms.
+        cut_to geq1; trivial.
+        generalize (nnrc_imp_stmt_eval_grouped_equiv geq1 h σc (nnrc_impish_stmt_to_nnrc_imp_stmt s1)); intros geq3.
+        rewrite eqq0 in geq3.
+        simpl in geq3.
+        match_option_in geq3; try contradiction.
+        simpl.
+        rewrite geq3 in IHs1.
+        rewrite H1 in *.
+        specialize (IHs2 ((s, o)::σ) _ _ sf2).
+        cut_to IHs2; [ | 
+                       rewrite all_disjoint3_iff in *
+                       ; repeat split; try tauto
+                       ; apply disjoint_cons1; tauto].
+        case_eq (nnrc_impish_stmt_eval h σc ((s, o) :: σ) m m0 s2)
+        ; [ intros ? eqq2 | intros eqq2]
+        ; rewrite eqq2 in *; simpl in *.
+        * match_option_in IHs2; try contradiction.
+          destruct p1 as [[??]?].
+          preserve_doms; simpl.
+          generalize (nnrc_imp_stmt_eval_grouped_equiv IHs1 h σc (nnrc_impish_stmt_to_nnrc_imp_stmt s2)); intros geq4.
+          rewrite eqq3 in geq4; simpl in geq4.
+          match_option_in geq4; try contradiction.
+          rewrite geq4 in IHs2.
+          generalize (nnrc_imp_stmt_eval_env_domain_stack eqq1)
+          ; intros deq1.
+          generalize (nnrc_imp_stmt_eval_env_domain_stack eqq4)
+          ; intros deq2.
+          rewrite deq2 in deq1.
+          simpl in deq1.
+          destruct p1; invcs deq1.
+          destruct p1; simpl in *.
+          apply grouped_equiv_cons_invs in IHs2.
+          tauto.
+        * match_option_in IHs2; try contradiction.
+          generalize (nnrc_imp_stmt_eval_grouped_equiv IHs1 h σc (nnrc_impish_stmt_to_nnrc_imp_stmt s2)); intros geq4.
+          rewrite eqq3 in geq4; simpl in *.
+          match_option_in geq4; try contradiction.
+      + apply none_lift in eqq.
+        rewrite eqq; simpl.
+        generalize (grouped_equiv_mdenv_env (v,None) σ ψc ψd); simpl
+        ; intros geq1.
+        cut_to geq1; trivial.
+        generalize (nnrc_imp_stmt_eval_grouped_equiv geq1 h σc (nnrc_impish_stmt_to_nnrc_imp_stmt s1)); intros geq2.
+        unfold var in *.
+        rewrite eqq0 in geq2; simpl in *.
+        match_option_in geq2; try contradiction.
+    - Case "NNRCimpishLetMutColl"%string.
+      destruct sf as [nin1 [nin2 [nin3 [sf1 sf2]]]].
+      specialize (IHs1 _ ((v, [])::ψc) _ sf1).
+      cut_to IHs1; [ | 
+                     rewrite all_disjoint3_iff in *; simpl in *
+                     ; repeat split; try tauto
+                     ; try apply disjoint_cons1; try apply disjoint_cons2; tauto].
+      unfold lift2P in IHs1.
+      repeat match_option_in IHs1; try contradiction.
+      + apply some_lift in eqq.
+        destruct eqq as [[[??]?] eqq ?]; subst.
+        rewrite eqq.
+        preserve_doms.
+        generalize (nnrc_impish_stmt_eval_mcenv_domain_stack eqq)
+        ; destruct m; intros deq; invcs deq.
+        destruct p; simpl in *.
+        generalize (grouped_equiv_mcenv_env (s,nil) σ ψc ψd); simpl
+        ; intros geq1.
+        generalize (grouped_equiv_mcenv_env (s,l) σ m m0); simpl
+        ; intros geq2.
+        rewrite geq2 in IHs1 by trivial.
+        preserve_doms.
+        cut_to geq1; trivial.
+        generalize (nnrc_imp_stmt_eval_grouped_equiv geq1 h σc (nnrc_impish_stmt_to_nnrc_imp_stmt s1)); intros geq3.
+        rewrite eqq0 in geq3.
+        simpl in geq3.
+        match_option_in geq3; try contradiction.
+        simpl.
+        rewrite geq3 in IHs1.
+        rewrite H1 in *.
+        specialize (IHs2 ((s, (Some (dcoll l)))::σ) _ _ sf2).
+        cut_to IHs2; [ | 
+                       rewrite all_disjoint3_iff in *
+                       ; repeat split; try tauto
+                       ; apply disjoint_cons1; tauto].
+        case_eq (nnrc_impish_stmt_eval h σc ((s, (Some (dcoll l))) :: σ) m m0 s2)
+        ; [ intros ? eqq2 | intros eqq2]
+        ; rewrite eqq2 in *; simpl in *.
+        * match_option_in IHs2; try contradiction.
+          destruct p1 as [[??]?].
+          preserve_doms; simpl.
+          generalize (nnrc_imp_stmt_eval_grouped_equiv IHs1 h σc (nnrc_impish_stmt_to_nnrc_imp_stmt s2)); intros geq4.
+          rewrite eqq3 in geq4; simpl in geq4.
+          match_option_in geq4; try contradiction.
+          rewrite geq4 in IHs2.
+          generalize (nnrc_imp_stmt_eval_env_domain_stack eqq1)
+          ; intros deq1.
+          generalize (nnrc_imp_stmt_eval_env_domain_stack eqq4)
+          ; intros deq2.
+          rewrite deq2 in deq1.
+          simpl in deq1.
+          destruct p1; invcs deq1.
+          destruct p1; simpl in *.
+          apply grouped_equiv_cons_invs in IHs2.
+          tauto.
+        * match_option_in IHs2; try contradiction.
+          generalize (nnrc_imp_stmt_eval_grouped_equiv IHs1 h σc (nnrc_impish_stmt_to_nnrc_imp_stmt s2)); intros geq4.
+          rewrite eqq3 in geq4; simpl in *.
+          match_option_in geq4; try contradiction.
+      + apply none_lift in eqq.
+        rewrite eqq; simpl.
+        generalize (grouped_equiv_mcenv_env (v,nil) σ ψc ψd); simpl
+        ; intros geq1.
+        cut_to geq1; trivial.
+        generalize (nnrc_imp_stmt_eval_grouped_equiv geq1 h σc (nnrc_impish_stmt_to_nnrc_imp_stmt s1)); intros geq2.
+        unfold var in *.
+        simpl in *.
+        rewrite eqq0 in geq2; simpl in *.
+        match_option_in geq2; try contradiction.
+    - Case "NNRCimpishAssign"%string.
+      destruct sf as [disj1 [disj2 [nin1 nin2]]].
+      rewrite <- nnrc_impish_expr_to_nnrc_imp_expr_correct.
+      rewrite nnrc_impish_expr_eval_free_env, nnrc_impish_expr_eval_free_env_tail           by (try rewrite domain_map_codomain; tauto).
+      match_option; simpl; trivial.
+      repeat rewrite lookup_app.
+      rewrite (lookup_nin_none _ nin1).
+      rewrite (@lookup_nin_none _ _ _ (map_codomain (fun x : list data => Some (dcoll x)) ψc))
+        by (try rewrite domain_map_codomain; trivial).
+      match_option; simpl; trivial.
+      repeat rewrite update_app_nin by (try rewrite domain_map_codomain; trivial).
+      reflexivity.
+    - Case "NNRCimpishPush"%string.
+      destruct sf as [disj1 [disj2 [nin1 nin2]]].
+      rewrite <- nnrc_impish_expr_to_nnrc_imp_expr_correct.
+      rewrite nnrc_impish_expr_eval_free_env, nnrc_impish_expr_eval_free_env_tail           by (try rewrite domain_map_codomain; tauto).
+      match_option; simpl; trivial; [ | rewrite olift2_none_r; trivial].
+      repeat rewrite lookup_app.
+      repeat rewrite (lookup_nin_none _ nin1).
+      rewrite (lookup_nin_none _ nin2).
+      repeat rewrite lookup_map_codomain.
+      unfold equiv_dec, string_eqdec.
+      match_option; simpl; trivial.
+      rewrite (update_app_nin string_dec σ) by trivial.
+      rewrite map_codomain_update_first; simpl.
+      rewrite update_app_nin2 by trivial.
+      unfold bunion.
+      apply grouped_equiv_equiv.
+    - Case "NNRCimpishFor"%string.
+      destruct sf as [disj1 [disj2 [nin1 [nin2 sf]]]].
+      rewrite <- nnrc_impish_expr_to_nnrc_imp_expr_correct.
+      rewrite nnrc_impish_expr_eval_free_env, nnrc_impish_expr_eval_free_env_tail           by (try rewrite domain_map_codomain; tauto).
+      match_option; simpl; trivial.
+      destruct d; simpl; trivial.
+      clear eqq.
+      revert σ ψc ψd disj disj1 disj2 nin1 nin2 sf IHs.
+      induction l; simpl; intros σ ψc ψd disj disj1 disj2 nin1 nin2 sf IHs; [reflexivity | ].
+      generalize IHs; intros IHsH.
+      specialize (IHs ((v,Some a)::σ) _ _ sf).
+      cut_to IHs
+      ; [ | rewrite all_disjoint3_iff in *
+          ; repeat split; try tauto
+          ; apply disjoint_cons1; tauto].
+      unfold var in *.
+      match_option
+      ; rewrite eqq in IHs; simpl in IHs
+      ; match_option_in IHs; try contradiction.
+      destruct p as [[??]?].
+      generalize (nnrc_impish_stmt_eval_env_stack eqq); intros; subst.
+      generalize (nnrc_imp_stmt_eval_env_domain_stack eqq0)
+      ; intros deq1.
+      simpl in deq1.
+      destruct p0; invcs deq1.
+      destruct p; simpl in *.
+      apply grouped_equiv_cons_invs in IHs.
+      destruct IHs as [? geq1]; subst.
+      preserve_doms.
+      rewrite IHl; trivial.
+      revert geq1.
+      generalize (σ ++ map_codomain (fun x : list data => Some (dcoll x)) m ++ m0).
+      clear.
+      revert p0.
+      induction l; simpl; trivial; intros p2 p1 geq1.
+      assert (geq2: grouped_equiv ((s0, Some a)::p1) ((s0, Some a) :: p2)).
+      { apply grouped_equiv_cons; trivial. }
+      generalize (nnrc_imp_stmt_eval_grouped_equiv
+                    geq2 h σc
+                    (nnrc_impish_stmt_to_nnrc_imp_stmt s))
+      ; intros geq3.
+      unfold var in *.
+      match_option; simpl in *
+      ; rewrite eqq in geq3; simpl in geq3
+      ; match_option_in geq3; try contradiction.
+      generalize (nnrc_imp_stmt_eval_env_domain_stack eqq)
+      ; intros deq1.
+      generalize (nnrc_imp_stmt_eval_env_domain_stack eqq0)
+      ; intros deq2.
+      simpl in deq1, deq2.
+      destruct p; invcs deq1.
+      destruct p0; invcs deq2.
+      destruct p; destruct p0; simpl in *; subst.
+      apply grouped_equiv_cons_invs in geq3.
+      apply IHl; tauto.
+    - Case "NNRCimpishIf"%string.
+      destruct sf as [disj1 [disj2 [sf1 sf2]]].
+      rewrite <- nnrc_impish_expr_to_nnrc_imp_expr_correct.
+      rewrite nnrc_impish_expr_eval_free_env, nnrc_impish_expr_eval_free_env_tail           by (try rewrite domain_map_codomain; tauto).
+      match_option; simpl; trivial.
+      destruct d; simpl; trivial.
+      destruct b; simpl; auto.
+    - Case "NNRCimpishEither"%string.
+      destruct sf as [disj1 [disj2 [nin1 [nin2 [nin3 [nin4 [sf1 sf2]]]]]]].
+      rewrite <- nnrc_impish_expr_to_nnrc_imp_expr_correct.
+      rewrite nnrc_impish_expr_eval_free_env, nnrc_impish_expr_eval_free_env_tail           by (try rewrite domain_map_codomain; tauto).
+      match_option; simpl; trivial.
+      destruct d; simpl; trivial.
+      + specialize (IHs1 ((v,Some d)::σ) _ _ sf1).
+        cut_to IHs1
+        ; [ | 
+            rewrite all_disjoint3_iff in *
+            ; repeat split; try tauto
+            ; apply disjoint_cons1; tauto].
+        unfold lift2P in IHs1.
+        unfold var in *.
+        match_option
+        ; rewrite eqq0 in IHs1; simpl in IHs1
+        ; match_option_in IHs1; try contradiction; simpl in *.
+        destruct p as [[??]?].
+        generalize (nnrc_impish_stmt_eval_env_stack eqq0); intros; subst.
+        generalize (nnrc_imp_stmt_eval_env_domain_stack eqq1)
+        ; intros deq1.
+        simpl in deq1.
+        destruct p0; invcs deq1.
+        destruct p; simpl in *.
+        apply grouped_equiv_cons_invs in IHs1.
+        tauto.
+      + specialize (IHs2 ((v0,Some d)::σ) _ _ sf2).
+        cut_to IHs2
+        ; [ | 
+            rewrite all_disjoint3_iff in *
+            ; repeat split; try tauto
+            ; apply disjoint_cons1; tauto].
+        unfold lift2P in IHs2.
+        unfold var in *.
+        match_option
+        ; rewrite eqq0 in IHs2; simpl in IHs2
+        ; match_option_in IHs2; try contradiction; simpl in *.
+        destruct p as [[??]?].
+        generalize (nnrc_impish_stmt_eval_env_stack eqq0); intros; subst.
+        generalize (nnrc_imp_stmt_eval_env_domain_stack eqq1)
+        ; intros deq1.
+        simpl in deq1.
+        destruct p0; invcs deq1.
+        destruct p; simpl in *.
+        apply grouped_equiv_cons_invs in IHs2.
+        tauto.
+  Qed.
+  
+  Theorem nnrc_impish_to_nnrc_imp_correct (s:nnrc_impish) :
+    forall h σc,
+      nnrc_impish_cross_shadow_free s ->
+      nnrc_impish_eval h σc s = nnrc_imp_eval h σc (nnrc_impish_to_nnrc_imp s).
+  Proof.
+    unfold nnrc_impish_cross_shadow_free.
+    intros h σc sf.
+    destruct s as [s ret].
+    generalize (nnrc_impish_stmt_to_nnrc_imp_stmt_correct s h σc nil nil ((ret,None)::nil)); simpl; intros HH.
+    cut_to HH; trivial.
+    - unfold var in *; match_option
+      ; rewrite eqq in HH; simpl in HH.
+      + match_option_in HH; try contradiction.
+        destruct p as [[??]?].
+        preserve_doms.
+        generalize (nnrc_impish_stmt_eval_mcenv_domain_stack eqq)
+        ; intros deq1.
+        generalize (nnrc_impish_stmt_eval_mdenv_domain_stack eqq)
+        ; intros deq2.
+        generalize (nnrc_imp_stmt_eval_env_domain_stack eqq0)
+        ; intros deq3.
+        destruct m0; simpl in *; invcs deq2.
+        destruct p0; simpl in *; invcs deq3.
+        symmetry in H1; apply domain_nil in H1.
+        symmetry in H2; apply domain_nil in H2.
+        symmetry in deq1; apply domain_nil in deq1.
+        subst.
+        simpl in *.
+        apply grouped_equiv_singleton in HH.
+        invcs HH.
+        trivial.
+      + match_option_in HH; try contradiction.
+    - apply all_disjoint3_iff; simpl.
+      eauto.
+  Qed.
+
+  Section Core.
+
+    Lemma nnrc_impish_expr_to_nnrc_imp_expr_preserves_core {e:nnrc_impish_expr} :
+      nnrc_impish_exprIsCore e <->
+      nnrc_imp_exprIsCore (nnrc_impish_expr_to_nnrc_imp_expr e).
+    Proof.
+      induction e; simpl; tauto.
+    Qed.
+
+    Lemma nnrc_impish_stmt_to_nnrc_imp_stmt_preserves_core {s:nnrc_impish_stmt} :
+      nnrc_impish_stmtIsCore s <->
+      nnrc_imp_stmtIsCore (nnrc_impish_stmt_to_nnrc_imp_stmt s).
+    Proof.
+      induction s; simpl;
+        repeat rewrite nnrc_impish_expr_to_nnrc_imp_expr_preserves_core
+        ; tauto.
+    Qed.
+
+    Theorem nnrc_impish_to_nnrc_imp_preserves_core {s:nnrc_impish} :
+      nnrc_impishIsCore s <->
+      nnrc_impIsCore (nnrc_impish_to_nnrc_imp s).
+    Proof.
+      destruct s; simpl.
+      apply nnrc_impish_stmt_to_nnrc_imp_stmt_preserves_core.
+    Qed.
+
+    (*
+    Theorem nnrc_impish_to_nnrc_imp_top_preserves_core {s:nnrc_impish} :
+      nnrc_impishIsCore s <->
+      nnrc_impIsCore (nnrc_impish_to_nnrc_imp_top s).
+    Proof.
+      unfold nnrc_to_nnrc_impish_top.
+      rewrite <- nnrc_impish_to_nnrc_imp_preserves_core.
+      apply stratify_preserves_core.
+    Qed.
+
+    Program Definition nnrc_impish_core_to_nnrc_imp_core_top
+            (s:nnrc_impish_core) : nnrc_imp_core
+      :=nnrc_impish_to_nnrc_imp_top s.
+    Next Obligation.
+      destruct s; simpl.
+      apply nnrc_impish_to_nnrc_imp_top_preserves_core; trivial.
+    Qed.
+
+    Theorem nnrc_impish_core_to_nnrc_imp_core_correct
+            h σc (s:nnrc_impish_core) :
+      nnrc_impish_core_eval_top h σc s
+      = nnrc_imp_core_eval_top h σc (nnrc_impish_core_to_nnrc_imp_core_top s).
+    Proof.
+      destruct s as [q pf].
+      generalize (nnrc_impish_to_nnrc_imp_correct h σc q); intros HH.
+      unfold nnrc_eval_top in HH.
+      rewrite <- nnrc_to_nnrc_ext_eq in HH by trivial.
+      unfold nnrc_core_eval_top, lift_nnrc_core; simpl.
+      rewrite HH.
+      reflexivity.
+    Qed.
+*)
+  End Core.
+
+End NNRCimpishtoNNRCimp.
